Add automatic properties for value maintenance

ind/DoublyLinkedListIface.fst
@@ -404,6 +404,19 @@ let auto_node_remains_valid_upon_staying_unchanged h0 h1 l n = ()
 
 let auto_dll_fp_upon_staying_unchanged h0 h1 l d = ()
 
+/// Automatic value maintenance
+///
+/// These are lemmas that you shouldn't really need to refer to
+/// manually. If you do, it is (likely) a bug wrt the patterns, and
+/// you should ask someone who knows about how this library works to
+/// look at things.
+
+let auto_dll_as_list_staying_unchanged h0 h1 l d =()
+
+let auto_node_val_staying_unchanged h0 h1 l n = ()
+
+let auto_node_val_unchanged_staying_unchanged h0 h1 n =()
+
 /// Properties of nodes inside and outside lists
 ///
 /// These are lemmas that you shouldn't really need to refer to
